Prove is_unique (needed for get_mut) for Arc.

theories/lang/lib/arc.v
@@ -22,7 +22,11 @@ Definition clone_weak : val :=
 Definition downgrade : val :=
   rec: "downgrade" ["l"] :=
     let: "weak" := !ˢᶜ("l" +ₗ #1) in
-    if: CAS ("l" +ₗ #1) "weak" ("weak" + #1) then #() else "downgrade" ["l"].
+    if: "weak" = #(-1) then
+      "downgrade" ["l"]
+    else
+      if: CAS ("l" +ₗ #1) "weak" ("weak" + #1) then #()
+      else "downgrade" ["l"].
 
 Definition upgrade : val :=
   rec: "upgrade" ["l"] :=
@@ -59,10 +63,25 @@ Definition try_unwrap_full : val :=
       else "l" <- #1;; #1
     else #2.
 
+Definition is_unique : val :=
+  λ: ["l"],
+    if: CAS ("l" +ₗ #1) #1 #(-1) then
+      let: "strong" := !ˢᶜ"l" in
+      let: "unique" := "strong" = #1 in
+      "l" +ₗ #1 <-ˢᶜ #1;;
+      "unique"
+    else
+      #false.
+
 (** The CMRA we need. *)
 (* Not bundling heapG, as it may be shared with other users. *)
+
+(* See rc.v for understanding the structure of this CMRA.
+   The only additional thing is the [optionR (exclR unitC))], used to handle
+   properly the locking mechanisme for the weak count. *)
 Definition arc_stR :=
-  prodUR (optionUR (csumR (prodR fracR positiveR) (exclR unitC))) natUR.
+  prodUR (optionUR (csumR (prodR (prodR fracR positiveR) (optionR (exclR unitC)))
+                          (exclR unitC))) natUR.
 Class arcG Σ :=
   RcG :> inG Σ (authR arc_stR).
 Definition arcΣ : gFunctors := #[GFunctor (authR arc_stR)].
@@ -73,7 +92,7 @@ Section def.
   Context `{!lrustG Σ, !arcG Σ} (P1 : Qp → iProp Σ) (P2 : iProp Σ) (N : namespace).
 
   Definition arc_tok γ q : iProp Σ :=
-    own γ (◯ (Some $ Cinl (q, 1%positive), 0%nat)).
+    own γ (◯ (Some $ Cinl (q, 1%positive, None), 0%nat)).
   Definition weak_tok γ : iProp Σ :=
     own γ (◯ (None, 1%nat)).
 
@@ -83,9 +102,10 @@ Section def.
   Definition arc_inv (γ : gname) (l : loc) : iProp Σ :=
     (∃ st : arc_stR, own γ (● st) ∗
       match st with
-      | (Some (Cinl (q, strong)), weak) => ∃ q',
-        l ↦ #(Zpos strong) ∗ shift_loc l 1 ↦ #(S weak) ∗
-          ⌜(q + q')%Qp = 1%Qp⌝ ∗ P1 q'
+      | (Some (Cinl (q, strong, wlock)), weak) =>
+         ∃ q', ⌜(q + q')%Qp = 1%Qp⌝ ∗ P1 q' ∗ l ↦ #(Zpos strong) ∗
+           if wlock then shift_loc l 1 ↦ #(-1) ∗ ⌜weak = 0%nat⌝
+           else shift_loc l 1 ↦ #(S weak)
       | (Some (Cinr _), weak) =>
         l ↦ #0 ∗ shift_loc l 1 ↦ #(S weak)
       | (None, (S _) as weak) =>
@@ -141,8 +161,9 @@ Section arc.
       ∃ γ q, is_arc P1 P2 N γ l ∗ P1 q ∗ arc_tok γ q.
   Proof using HP1.
     iIntros "Hl1 Hl2 [HP1 HP1']".
-    iMod (own_alloc ((● (Some $ Cinl ((1/2)%Qp, xH), O) ⋅
-                      ◯ (Some $ Cinl ((1/2)%Qp, xH), O)))) as (γ) "[H● H◯]"; first done.
+    iMod (own_alloc ((● (Some $ Cinl ((1/2)%Qp, xH, None), O) ⋅
+                      ◯ (Some $ Cinl ((1/2)%Qp, xH, None), O))))
+      as (γ) "[H● H◯]"; first done.
     iExists _, _. iFrame. iApply inv_alloc. iExists _. iFrame. iExists _. iFrame.
     rewrite Qp_div_2. auto.
   Qed.
@@ -157,19 +178,18 @@ Section arc.
 
   Lemma arc_tok_auth_val st γ q :
     own γ (● st) -∗ arc_tok γ q -∗
-    ⌜∃ q' strong weak, st = (Some $ Cinl (q', strong), weak) ∧
-                       if decide (strong = xH) then q = q'
-                        else ∃ q'', q' = (q + q'')%Qp⌝.
+    ⌜∃ q' strong wlock weak, st = (Some $ Cinl (q', strong, wlock), weak) ∧
+                             if decide (strong = xH) then q = q' ∧ wlock = None
+                             else ∃ q'', q' = (q + q'')%Qp⌝.
   Proof.
     iIntros "H● Htok". iDestruct (own_valid_2 with "H● Htok") as
         %[[Hincl%option_included _]%prod_included [Hval _]]%auth_valid_discrete_2.
     destruct st, Hincl as [[=]|(?&?&[= <-]&?&[Hincl|Hincl%csum_included])];
       simpl in *; subst.
-    - setoid_subst. iExists _, _, _. by iSplit.
-    - destruct Hincl as [->|[(?&[]&[=<-]&->&
-             [[??]%frac_included%Qp_lt_sum  ?%pos_included]%prod_included)|
-        (?&?&[=]&?)]]; first done.
-      iExists _, _, _. iSplit=>//. simpl in *. destruct decide; [subst;lia|eauto].
+    - setoid_subst. iExists _, _, _, _. by iSplit.
+    - destruct Hincl as [->|[(?&[[??]?]&[=<-]&->&[[[??]%frac_included%Qp_lt_sum
+        ?%pos_included]%prod_included _]%prod_included)|(?&?&[=]&?)]]; first done.
+      iExists _, _, _, _. iSplit=>//. simpl in *. destruct decide; [subst;lia|eauto].
   Qed.
 
   Lemma clone_arc_spec (γ : gname) (l : loc) (P : iProp Σ) :
@@ -180,30 +200,31 @@ Section arc.
     iIntros "#INV #Hacc !# * HP HΦ". iLöb as "IH". wp_rec. wp_bind (!ˢᶜ_)%E.
     iInv N as (st) "[>H● H]" "Hclose1".
     iMod ("Hacc" with "HP") as (?) "[Hown Hclose2]".
-    iDestruct (arc_tok_auth_val with "H● Hown") as %(?& strong &?&[-> _]).
-    iDestruct "H" as (?) "[H H']". wp_read. iMod ("Hclose2" with "Hown") as "HP".
-    iModIntro. iMod ("Hclose1" with "[H H' H●]") as "_".
-    { iExists _. auto with iFrame. }
+    iDestruct (arc_tok_auth_val with "H● Hown") as %(?& strong &?&?&[-> _]).
+    iDestruct "H" as (?) "(Hq & HP1 & H↦ & Hw)". wp_read.
+    iMod ("Hclose2" with "Hown") as "HP". iModIntro.
+    iMod ("Hclose1" with "[-HP HΦ]") as "_"; [iExists _; auto with iFrame|].
     iModIntro. wp_let. wp_op. wp_bind (CAS _ _ _). iInv N as (st) "[>H● H]" "Hclose1".
     iMod ("Hacc" with "HP") as (?) "[Hown Hclose2]".
-    iDestruct (arc_tok_auth_val with "H● Hown") as %(?&strong'&?&[-> _]).
-    iDestruct "H" as (q) "(Hl & Hl1 & >Heq & [HP1 HP1'])". iDestruct "Heq" as %Heq.
+    iDestruct (arc_tok_auth_val with "H● Hown") as %(?&strong'&?&?&[-> _]).
+    iDestruct "H" as (q) "(>#Hq & [HP1 HP1'] & Hl & Hw)". iDestruct "Hq" as %Hq.
     destruct (decide (strong = strong')) as [->|?].
     - wp_apply (wp_cas_int_suc with "Hl"); first done. iIntros "Hl".
       iMod (own_update with "H●") as "[H● Hown']".
       { apply auth_update_alloc, prod_local_update_1,
-         (op_local_update_discrete _ _ (Some (Cinl ((q/2)%Qp, 1%positive))))=>-[/= Hqa _].
-        split; simpl; last done. apply frac_valid'. rewrite -Heq comm_L -{2}(Qp_div_2 q).
+         (op_local_update_discrete _ _ (Some (Cinl ((q/2)%Qp, 1%positive, None))))
+           =>-[/= Hqa ?]. split;[split|]=>//=; last by rewrite left_id.
+        apply frac_valid'. rewrite -Hq comm_L -{2}(Qp_div_2 q).
         apply Qcplus_le_mono_l. rewrite -{1}(Qcplus_0_l (_ / _)%Qp).
         apply Qcplus_le_mono_r, Qp_ge_0. }
       iMod ("Hclose2" with "Hown") as "HP". iModIntro.
-      iMod ("Hclose1" with "[Hl Hl1 H● HP1']") as "_".
+      iMod ("Hclose1" with "[Hl Hw H● HP1']") as "_".
       { iExists _. iFrame. iExists _. rewrite /= [xH ⋅ _]comm_L. iFrame.
-        rewrite [(q / 2)%Qp ⋅ _]comm frac_op' -[(_ + _)%Qp]assoc Qp_div_2. auto. }
+        rewrite [(q / 2)%Qp ⋅ _]comm frac_op' -[(_ + _)%Qp]assoc Qp_div_2 left_id_L. auto. }
       iModIntro. wp_apply (wp_if _ true). wp_value. iApply "HΦ". iFrame.
     - wp_apply (wp_cas_int_fail with "Hl"); [done|congruence|]. iIntros "Hl".
       iMod ("Hclose2" with "Hown") as "HP". iModIntro.
-      iMod ("Hclose1" with "[Hl Hl1 HP1 HP1' H●]") as "_".
+      iMod ("Hclose1" with "[-HP HΦ]") as "_".
       { iExists _. iFrame. iExists q. auto with iFrame. }
       iModIntro. wp_apply (wp_if _ false). iApply ("IH" with "HP HΦ").
   Qed.
@@ -214,32 +235,40 @@ Section arc.
   Proof.
     iIntros "#INV #Hacc !# * HP HΦ". iLöb as "IH". wp_rec. wp_op. wp_bind (!ˢᶜ_)%E.
     iInv N as (st) "[>H● H]" "Hclose1".
-    iMod ("Hacc" with "HP") as (?) "[Hown Hclose2]".
-    iDestruct (arc_tok_auth_val with "H● Hown") as %(?&?& weak &[-> _]).
-    iDestruct "H" as (?) "(H & H' & H'')". wp_read. iMod ("Hclose2" with "Hown") as "HP".
-    iModIntro. iMod ("Hclose1" with "[H H' H'' H●]") as "_".
-    { iExists _. auto with iFrame. }
-    iModIntro. wp_let. wp_op. wp_bind (CAS _ _ _). wp_op.
+    iApply fupd_wp. iMod ("Hacc" with "HP") as (?) "[Hown Hclose2]".
+    iDestruct (arc_tok_auth_val with "H● Hown") as %(?&?& wlock & weak &[-> _]).
+    iMod ("Hclose2" with "Hown") as "HP". iModIntro.
+    iDestruct "H" as (?) "(? & ? & ? & Hw)". destruct wlock.
+    { iDestruct "Hw" as "(Hw & >%)". subst. wp_read.
+      iMod ("Hclose1" with "[-HP HΦ]") as "_"; first by iExists _; auto with iFrame.
+      iModIntro. wp_let. wp_op=>[_|//]. wp_if. iApply ("IH" with "HP HΦ"). }
+    wp_read. iMod ("Hclose1" with "[-HP HΦ]") as "_"; first by iExists _; auto with iFrame.
+    iModIntro. wp_let. wp_op=>[//|_]. wp_if. wp_op. wp_op. wp_bind (CAS _ _ _).
     iInv N as (st) "[>H● H]" "Hclose1".
-    iMod ("Hacc" with "HP") as (?) "[Hown Hclose2]".
-    iDestruct (arc_tok_auth_val with "H● Hown") as %(?&?& weak' &[-> _]).
-    iDestruct "H" as (q) "(Hl & Hl1 & >Heq & HP1)". iDestruct "Heq" as %Heq.
-    destruct (decide (weak = weak')) as [<-|Hw].
+    iApply fupd_wp. iMod ("Hacc" with "HP") as (?) "[Hown Hclose2]".
+    iDestruct (arc_tok_auth_val with "H● Hown") as %(?&?& wlock & weak' &[-> _]).
+    iMod ("Hclose2" with "Hown") as "HP". iModIntro.
+    iDestruct "H" as (q) "(>Heq & HP1 & Hl & Hl1)". iDestruct "Heq" as %Heq.
+    destruct (decide (weak = weak' ∧ wlock = None)) as [[<- ->]|Hw].
     - wp_apply (wp_cas_int_suc with "Hl1"); first done. iIntros "Hl1".
       iMod (own_update with "H●") as "[H● Hown']".
       { by apply auth_update_alloc, prod_local_update_2,
               (op_local_update_discrete _ _ (1%nat)). }
-      iMod ("Hclose2" with "Hown") as "HP". iModIntro.
-      iMod ("Hclose1" with "[Hl Hl1 H● HP1]") as "_".
+      iMod ("Hclose1" with "[-Hown' HP HΦ]") as "_".
       { iExists _. iFrame. iExists _.
         rewrite Z.add_comm (Nat2Z.inj_add 1). auto with iFrame. }
       iModIntro. wp_apply (wp_if _ true). wp_value. iApply "HΦ". iFrame.
-    - wp_apply (wp_cas_int_fail with "Hl1"); [done| |].
-      { contradict Hw. apply SuccNat2Pos.inj. lia. }
-      iMod ("Hclose2" with "Hown") as "HP". iIntros "Hl1 !>".
-      iMod ("Hclose1" with "[Hl Hl1 HP1 H●]") as "_".
-      { iExists _. auto with iFrame. }
-      iModIntro. wp_apply (wp_if _ false). iApply ("IH" with "HP HΦ").
+    - destruct wlock.
+      + iDestruct "Hl1" as "[Hl1 >%]". subst.
+        wp_apply (wp_cas_int_fail with "Hl1"); [done..|].
+        iIntros "Hl1". iMod ("Hclose1" with "[-HP HΦ]") as "_".
+        { iExists _. auto with iFrame. }
+        iModIntro. wp_apply (wp_if _ false). iApply ("IH" with "HP HΦ").
+      + wp_apply (wp_cas_int_fail with "Hl1"); [done| |].
+        { contradict Hw. split=>//. apply SuccNat2Pos.inj. lia. }
+        iIntros "Hl1". iMod ("Hclose1" with "[-HP HΦ]") as "_".
+        { iExists _. auto with iFrame. }
+        iModIntro. wp_apply (wp_if _ false). iApply ("IH" with "HP HΦ").
   Qed.
 
   Lemma weak_tok_auth_val γ st :
@@ -256,31 +285,30 @@ Section arc.
     {{{ P }}} clone_weak [ #l] {{{ RET #(); P ∗ weak_tok γ }}}.
   Proof.
     iIntros "#INV #Hacc !# * HP HΦ". iLöb as "IH". wp_rec. wp_op. wp_bind (!ˢᶜ_)%E.
-    iAssert (□ (P ={⊤,∅}=∗ ∃ w : Z, shift_loc l 1 ↦ #w ∗
-              (shift_loc l 1 ↦ #(w + 1) ={∅,⊤}=∗ P ∗ weak_tok γ) ∧
-              (shift_loc l 1 ↦ #w ={∅,⊤}=∗ P)))%I as "#Hproto".
+    iAssert (□ (P ={⊤,⊤∖↑N}=∗ ∃ w : Z, shift_loc l 1 ↦ #w ∗
+              (shift_loc l 1 ↦ #(w + 1) ={⊤∖↑N,⊤}=∗ P ∗ weak_tok γ) ∧
+              (shift_loc l 1 ↦ #w ={⊤∖↑N,⊤}=∗ P)))%I as "#Hproto".
     { iIntros "!# HP". iInv N as (st) "[>H● H]" "Hclose1".
       iMod ("Hacc" with "HP") as "[Hown Hclose2]".
       iDestruct (weak_tok_auth_val with "H● Hown") as %(st' & weak & -> & Hval).
-      destruct st' as [[[]| |]|]; try done; iExists _.
-      - iDestruct "H" as (?) "(? & >$ & ?)". iIntros "!>"; iSplit; iIntros "?";
-        iMod ("Hclose2" with "Hown") as "HP".
+      iMod ("Hclose2" with "Hown") as "HP".
+      destruct st' as [[[[??][?|]]| |]|]; try done; [|iExists _..].
+      - by iDestruct "H" as (?) "(_ & _ & _ & _ & >%)".
+      - iDestruct "H" as (?) "(? & ? & ? & >$)". iIntros "!>"; iSplit; iIntros "?".
         + iMod (own_update with "H●") as "[H● $]".
           { by apply auth_update_alloc, prod_local_update_2,
                   (op_local_update_discrete _ _ (1%nat)). }
           rewrite Z.add_comm -(Nat2Z.inj_add 1). iFrame.
           iApply "Hclose1". iExists _. auto with iFrame.
         + iFrame. iApply ("Hclose1" with "[-]"). iExists _. auto with iFrame.
-      - iDestruct "H" as "[? >$]". iIntros "!>"; iSplit; iIntros "?";
-        iMod ("Hclose2" with "Hown") as "HP".
+      - iDestruct "H" as "[? >$]". iIntros "!>"; iSplit; iIntros "?".
         + iMod (own_update with "H●") as "[H● $]".
           { by apply auth_update_alloc, prod_local_update_2,
                   (op_local_update_discrete _ _ (1%nat)). }
           rewrite Z.add_comm -(Nat2Z.inj_add 1). iFrame. iApply "Hclose1".
           iExists _. auto with iFrame.
         + iFrame. iApply ("Hclose1" with "[-]"). iExists _. auto with iFrame.
-      - iDestruct "H" as "(? & >$ & ?)". iIntros "!>"; iSplit; iIntros "?";
-        iMod ("Hclose2" with "Hown") as "HP".
+      - iDestruct "H" as "(? & >$ & ?)". iIntros "!>"; iSplit; iIntros "?".
         + iMod (own_update with "H●") as "[H● $]".
           { by apply auth_update_alloc, prod_local_update_2,
                   (op_local_update_discrete _ _ (1%nat)). }
@@ -311,18 +339,19 @@ Section arc.
     { iIntros "!# HP". iInv N as (st) "[>H● H]" "Hclose1".
       iMod ("Hacc" with "HP") as "[Hown Hclose2]".
       iDestruct (weak_tok_auth_val with "H● Hown") as %(st' & weak & -> & Hval).
-      destruct st' as [[[]| |]|]; try done; iExists _.
-      - iDestruct "H" as (q) "(>$ & ? & >Heq & [HP1 HP1'])". iDestruct "Heq" as %Heq.
+      destruct st' as [[[[??]?]| |]|]; try done; iExists _.
+      - iDestruct "H" as (q) "(>Heq & [HP1 HP1'] & >$ & ?)". iDestruct "Heq" as %Heq.
         iIntros "!>"; iSplit; iMod ("Hclose2" with "Hown") as "HP".
         + iIntros "_ Hl". iExists (q/2)%Qp. iMod (own_update with "H●") as "[H● $]".
           { apply auth_update_alloc. rewrite -[(_,0%nat)]right_id.
-            apply op_local_update_discrete. constructor; last done. split; last done.
+            apply op_local_update_discrete=>Hv. constructor; last done.
+            split; last by rewrite /= left_id; apply Hv. split=>[|//].
             apply frac_valid'. rewrite -Heq comm_L -{2}(Qp_div_2 q).
             apply Qcplus_le_mono_l. rewrite -{1}(Qcplus_0_l (_ / _)%Qp).
             apply Qcplus_le_mono_r, Qp_ge_0. }
           iFrame. iApply "Hclose1". iExists _. iFrame. iExists _. iFrame.
           rewrite /= [xH ⋅ _]comm_L frac_op' [(_ + c)%Qp]comm -[(_ + _)%Qp]assoc
-                  Qp_div_2. auto with iFrame.
+                  Qp_div_2 left_id_L. auto with iFrame.
         + iIntros "Hl". iFrame. iApply ("Hclose1" with "[-]"). iExists _. iFrame.
           iExists q. auto with iFrame.
       - iDestruct "H" as "[>$ ?]". iIntros "!>"; iSplit; first by auto with congruence.
@@ -357,8 +386,9 @@ Section arc.
               (shift_loc l 1 ↦ #w ={⊤ ∖ ↑N,⊤}=∗ weak_tok γ)))%I as "#Hproto".
     { iIntros "!# Hown". iInv N as (st) "[>H● H]" "Hclose1".
       iDestruct (weak_tok_auth_val with "H● Hown") as %(st' & weak & -> & Hval).
-      destruct st' as [[[]| |]|]; try done; iExists _.
-      - iDestruct "H" as (q) "(? & >$ & >Heq & HP1)". iIntros "!>"; iSplit; iIntros "Hl1".
+      destruct st' as [[[[??][?|]]| |]|]; try done; [|iExists _..].
+      - by iDestruct "H" as (?) "(_ & _ & _ & _ & >%)".
+      - iDestruct "H" as (q) "(>Heq & HP1 & ? & >$)". iIntros "!>"; iSplit; iIntros "Hl1".
         + iMod ("Hclose1" with "[>-]") as "_"; last iLeft; auto with lia.
           iExists _. iMod (own_update_2 with "H● Hown") as "$".
           { apply auth_update_dealloc, prod_local_update_2,
@@ -377,7 +407,7 @@ Section arc.
           { apply auth_update_dealloc, prod_local_update_2,
                   (cancel_local_update_empty 1%nat), _. }
           destruct weak as [|weak].
-          * iMod ("Hclose1" with "[-HP2 H Hl1]") as "_"; last by auto with iFrame.
+          * iMod ("Hclose1" with "[H●]") as "_"; last by auto with iFrame.
             iExists _. iFrame.
           * iMod ("Hclose1" with "[>-]") as "_"; last iLeft; auto with lia.
             iExists _. iFrame. by replace (S (S weak) - 1) with (S weak:Z) by lia.
@@ -403,17 +433,17 @@ Section arc.
   Proof using HP1.
     iIntros "#INV #Hdrop #Hdealloc !# * (HP & Hown & HP1) HΦ". iLöb as "IH".
     wp_rec. wp_bind (!ˢᶜ_)%E. iInv N as (st) "[>H● H]" "Hclose".
-    iDestruct (arc_tok_auth_val with "H● Hown") as %(?& s &?&[-> _]).
-    iDestruct "H" as (?) "[H H']". wp_read. iMod ("Hclose" with "[H H' H●]") as "_".
-    { iExists _. auto with iFrame. }
+    iDestruct (arc_tok_auth_val with "H● Hown") as %(?& s &?&?&[-> _]).
+    iDestruct "H" as (?) "(? & ? & ? & ?)". wp_read.
+    iMod ("Hclose" with "[-HP Hown HP1 HΦ]") as "_". { iExists _. auto with iFrame. }
     iModIntro. wp_let. wp_op. wp_bind (CAS _ _ _).
     iInv N as (st) "[>H● H]" "Hclose".
-    iDestruct (arc_tok_auth_val with "H● Hown") as %(q' & s' & w &[-> Hqq']).
-    iDestruct "H" as (q'') "(Hs & Hw & >Hq'' & HP1')". iDestruct "Hq''" as %Hq''.
+    iDestruct (arc_tok_auth_val with "H● Hown") as %(q' & s' & wl & w &[-> Hqq']).
+    iDestruct "H" as (q'') "(>Hq'' & HP1' & Hs & Hw)". iDestruct "Hq''" as %Hq''.
     destruct (decide (s = s')) as [<-|?].
     - wp_apply (wp_cas_int_suc with "Hs"); first done. iIntros "Hs".
       destruct decide as [->|?].
-      + revert Hq''. rewrite -Hqq' // => Hq''.
+      + destruct Hqq' as [<- ->].
         iMod (own_update_2 with "H● Hown") as "[H● H◯]".
         { apply auth_update, prod_local_update_1. rewrite -[x in (x, _)]right_id.
           etrans; first apply cancel_local_update_empty, _.
@@ -432,11 +462,12 @@ Section arc.
           apply delete_option_local_update, _. }
         iFrame. iApply "Hclose". iExists _. by iFrame.
       + destruct Hqq' as [? ->].
-        rewrite -[in (_, _)](Pos.succ_pred s) // -Pos.add_1_l -pair_op -Cinl_op Some_op.
+        rewrite -[in (_, _)](Pos.succ_pred s) // -[wl in Cinl (_, wl)]left_id
+                -Pos.add_1_l -2!pair_op -Cinl_op Some_op.
         iMod (own_update_2 _ _ _ _ with "H● Hown") as "H●".
         { apply auth_update_dealloc, prod_local_update_1, @cancel_local_update_empty, _. }
         iMod ("Hclose" with "[- HΦ HP]") as "_".
-        { iExists _. iFrame. iExists (q + q'')%Qp. iFrame. iSplit; first by destruct s.
+        { iExists _. iFrame. iExists (q + q'')%Qp. iFrame. iSplit; last by destruct s.
           iIntros "!> !%". rewrite assoc -Hq''. f_equal. apply comm, _. }
         iModIntro. wp_apply (wp_if _ true). wp_op. by intros [=->]. intros _.
         wp_if. by iApply "HΦ".
@@ -453,12 +484,11 @@ Section arc.
         if b then P1 1 ∗ (P2 ={⊤}=∗ weak_tok γ) else arc_tok γ q ∗ P1 q }}}.
   Proof using HP1.
     iIntros "#INV !# * [Hown HP1] HΦ". wp_rec. iInv N as (st) "[>H● H]" "Hclose".
-    iDestruct (arc_tok_auth_val with "H● Hown") as %(q' & s & w &[-> Hqq']).
-    iDestruct "H" as (q'') "(Hs & Hw & >Hq'' & HP1')". iDestruct "Hq''" as %Hq''.
+    iDestruct (arc_tok_auth_val with "H● Hown") as %(q' & s & wl & w &[-> Hqq']).
+    iDestruct "H" as (q'') "(>Hq'' & HP1' & Hs & Hw)". iDestruct "Hq''" as %Hq''.
     destruct (decide (s = xH)) as [->|?].
     - wp_apply (wp_cas_int_suc with "Hs"); first done. iIntros "Hs".
-      revert Hq''. rewrite -Hqq' // => Hq''.
-      iMod (own_update_2 with "H● Hown") as "[H● H◯]".
+      destruct Hqq' as [<- ->]. iMod (own_update_2 with "H● Hown") as "[H● H◯]".
       { apply auth_update, prod_local_update_1. rewrite -[x in (x, _)]right_id.
         etrans; first apply cancel_local_update_empty, _.
         by apply (op_local_update _ _ (Some (Cinr (Excl ())))). }
@@ -474,18 +504,70 @@ Section arc.
         apply delete_option_local_update, _. }
       iApply "Hclose". iExists _. by iFrame.
     - wp_apply (wp_cas_int_fail with "Hs"); [done|congruence|]. iIntros "Hs".
-      iMod ("Hclose" with "[Hs Hw HP1' H●]") as "_"; first by iExists _; auto with iFrame.
+      iMod ("Hclose" with "[-Hown HP1 HΦ]") as "_"; first by iExists _; auto with iFrame.
       iApply ("HΦ" $! false). by iFrame.
   Qed.
 
-  (* Lemma try_unwrap_spec (γ : gname) (q: Qp) (l : loc) : *)
-  (*   is_arc γ l -∗ *)
-  (*   {{{ own γ (arc_tok q) ∗ P1 q }}} get_mut [ #l] *)
-  (*   {{{ (b : bool), RET #b ; *)
-  (*       if b then P1 1 ∗ (P1 1 ={⊤}=∗ ∃ γ' q', own γ' (arc_tok q') ∗ P1 q') *)
-  (*       else own γ (arc_tok q) ∗ P1 q }}}. *)
-  (* Proof. *)
-
+  Lemma is_unique_spec (γ : gname) (q: Qp) (l : loc) :
+    is_arc P1 P2 N γ l -∗
+    {{{ arc_tok γ q ∗ P1 q }}} is_unique [ #l]
+    {{{ (b : bool), RET #b ;
+        if b then l ↦ #1 ∗ shift_loc l 1 ↦ #1 ∗ P1 1
+        else arc_tok γ q ∗ P1 q }}}.
+  Proof using HP1.
+    iIntros "#INV !# * [Hown HP1] HΦ". wp_rec. wp_bind (CAS _ _ _). wp_op.
+    iInv N as (st) "[>H● H]" "Hclose".
+    iDestruct (arc_tok_auth_val with "H● Hown") as %(? & ? & wl & w &[-> _]).
+    iDestruct "H" as (?) "(>Hq'' & HP1' & >Hs & >Hw)".
+    destruct wl; last (destruct w; last first).
+    - iDestruct "Hw" as "[Hw %]". subst.
+      iApply (wp_cas_int_fail with "Hw")=>//. iNext. iIntros "Hw".
+      iMod ("Hclose" with "[-HΦ Hown HP1]") as "_"; first by iExists _; eauto with iFrame.
+      iModIntro. iApply (wp_if _ false). iModIntro. wp_value. iApply "HΦ". iFrame.
+    - iApply (wp_cas_int_fail with "Hw"); [done|lia|]. iNext. iIntros "Hw".
+      iMod ("Hclose" with "[-HΦ Hown HP1]") as "_"; first by iExists _; eauto with iFrame.
+      iModIntro. iApply (wp_if _ false). iModIntro. wp_value. iApply "HΦ". iFrame.
+    - iApply (wp_cas_int_suc with "Hw")=>//. iNext. iIntros "Hw".
+      iMod (own_update_2 with "H● Hown") as "[H● H◯]".
+      { by apply auth_update, prod_local_update_1, option_local_update,
+                 csum_local_update_l, prod_local_update_2,
+                 (alloc_option_local_update (Excl ())). }
+      iMod ("Hclose" with "[-HΦ HP1 H◯]") as "_"; first by iExists _; eauto with iFrame.
+      iModIntro. iApply (wp_if _ true). iNext. wp_bind (!ˢᶜ_)%E.
+      iInv N as ([st ?]) "[>H● H]" "Hclose".
+      iDestruct (own_valid_2 with "H● H◯") as
+        %[[[[=]|Hincl]%option_included _]%prod_included [? _]]%auth_valid_discrete_2.
+      simpl in Hincl. destruct Hincl as (? & ? & [=<-] & -> & [|Hincl]); last first.
+      + apply csum_included in Hincl. destruct Hincl as [->|[Hincl|(?&?&[=]&?)]]=>//.
+        destruct Hincl as (?&[[??]?]&[=<-]&->&[[_ Hlt]%prod_included _]%prod_included).
+        simpl in Hlt. apply pos_included in Hlt.
+        iDestruct "H" as (?) "(? & ? & ? & ?)". wp_read.
+        iMod ("Hclose" with "[-HΦ H◯ HP1]") as "_"; first by iExists _; auto with iFrame.
+        iModIntro. wp_let. wp_op; [lia|intros _]. wp_let. wp_op. wp_bind (_ <-ˢᶜ _)%E.
+        iInv N as ([st w]) "[>H● H]" "Hclose".
+        iDestruct (own_valid_2 with "H● H◯") as
+           %[[[[=]|Hincl]%option_included _]%prod_included [Hval _]]%auth_valid_discrete_2.
+        simpl in Hincl. destruct Hincl as (? & ? & [=<-] & -> & Hincl); last first.
+        assert (∃ q p, x2 = Cinl (q, p, Excl' ())) as (? & ? & ->).
+        { destruct Hincl as [|Hincl]; first by setoid_subst; eauto.
+          apply csum_included in Hincl. destruct Hincl as [->|[Hincl|(?&?&[=]&?)]]=>//.
+          destruct Hincl as (?&[[??]?]&[=<-]&->&[_ Hincl%option_included]%prod_included).
+          simpl in Hincl. destruct Hincl as [[=]|(?&?&[=<-]&->&[?|[]%exclusive_included])];
+            [|by apply _|by apply Hval]. setoid_subst. eauto. }
+        iDestruct "H" as (?) "(? & ? & ? & >? & >%)". subst. wp_write.
+        iMod (own_update_2 with "H● H◯") as "[H● H◯]".
+        { apply auth_update, prod_local_update_1, option_local_update,
+          csum_local_update_l, prod_local_update_2, delete_option_local_update, _. }
+        iMod ("Hclose" with "[-HΦ H◯ HP1]") as "_"; first by iExists _; auto with iFrame.
+        iModIntro. wp_seq. iApply "HΦ". iFrame.
+      + setoid_subst. iDestruct "H" as (?) "(Hq & ? & ? & >? & >%)". subst. wp_read.
+        iMod (own_update_2 with "H● H◯") as "H●".
+        { apply auth_update_dealloc. rewrite -{1}[(_, 0%nat)]right_id.
+          apply cancel_local_update_empty, _. }
+        iMod ("Hclose" with "[H●]") as "_"; first by iExists _; iFrame.
+        iModIntro. wp_seq. wp_op=>[_|//]. wp_let. wp_op. wp_write. iApply "HΦ".
+        iDestruct "Hq" as %<-. iFrame.
+  Qed.
 End arc.
 
 Typeclasses Opaque is_arc arc_tok weak_tok.
